add Banach's fixpoint and Löb induction

HeapLang/WeakestPrecondition.thy
@@ -1,5 +1,5 @@
 theory WeakestPrecondition
-imports "../IrisCore/Invariant" "../IrisCore/AuthHeap" HeapLang State PrimitiveLaws
+imports "../IrisCore/Invariant" "../IrisCore/AuthHeap" HeapLang State PrimitiveLaws Notation
 begin
 
 subsection \<open>Weakest Preconditions\<close>
@@ -8,21 +8,66 @@ definition state_interp :: "state \<Rightarrow> observation list \<Rightarrow> i
   "state_interp \<sigma> \<kappa>s = heap_interp (heap \<sigma>) \<^emph> proph_map_interp \<kappa>s (used_proph_id \<sigma>)"
 
 datatype stuckness = NotStuck | MaybeStuck
+instantiation stuckness :: ord begin
+fun less_eq_stuckness :: "stuckness \<Rightarrow> stuckness \<Rightarrow> bool" where
+  "less_eq_stuckness MaybeStuck NotStuck = False"
+| "less_eq_stuckness _ _ = True"
+fun less_stuckness :: "stuckness \<Rightarrow> stuckness \<Rightarrow> bool" where
+  "less_stuckness MaybeStuck NotStuck = False"
+| "less_stuckness MaybeStuck MaybeStuck = False"
+| "less_stuckness NotStuck NotStuck = False"
+| "less_stuckness _ _ = True"
+instance ..
+end
 
 definition fill :: "ectx_item list \<Rightarrow> expr \<Rightarrow> expr"  where "fill K e =  fold fill_item K e"
 
-inductive prim_step :: "expr \<Rightarrow> state \<Rightarrow> observation list \<Rightarrow> expr \<Rightarrow> state \<Rightarrow> expr list \<Rightarrow> bool" where
-Ectx_step:  "\<lbrakk>e1=fill K e1'; e2=fill K e2'; head_step e1' \<sigma>1 \<kappa> e2' \<sigma>2 efs\<rbrakk> \<Longrightarrow>
-   prim_step e1 \<sigma>1 \<kappa> e2 \<sigma>2 efs"
+definition prim_step :: "expr \<Rightarrow> state \<Rightarrow> observation list \<Rightarrow> expr \<Rightarrow> state \<Rightarrow> expr list \<Rightarrow> bool" where
+  "prim_step e1 \<sigma>1 \<kappa> e2 \<sigma>2 efs \<equiv> \<exists>K e1' e2'. ((e1=fill K e1') \<and> (e2=fill K e2') \<and> head_step e1' \<sigma>1 \<kappa> e2' \<sigma>2 efs)"
 
 function wp :: "stuckness \<Rightarrow> mask \<Rightarrow> expr \<Rightarrow> (val \<Rightarrow> iprop) \<Rightarrow> iprop" where
-  "wp s E e1 \<Phi> = (case to_val e1 of Some v \<Rightarrow> (\<Turnstile>{E}=> (\<Phi> v))
+  "wp s E e1 \<Phi> = (case HeapLang.to_val e1 of Some v \<Rightarrow> \<Turnstile>{E}=> (\<Phi> v)
     | None \<Rightarrow> (\<forall>\<^sub>u \<sigma>1 \<kappa> \<kappa>s.
       ((state_interp \<sigma>1 (\<kappa>@\<kappa>s)) ={E,Set.empty}=\<^emph>
         ((\<upharpoonleft>(case s of NotStuck \<Rightarrow> red e1 \<sigma>1 | _ \<Rightarrow> True)) \<^emph>
         (\<forall>\<^sub>u e2 \<sigma>2 efs. ((\<upharpoonleft>(prim_step e1 \<sigma>1 \<kappa> e2 \<sigma>2 efs))
           ={Set.empty}\<triangleright>=\<^emph> (\<Turnstile>{Set.empty,E}=> ((state_interp \<sigma>2 \<kappa>s) \<^emph>
             (wp s E e2 \<Phi>) \<^emph> ([\<^emph>\<^sub>l:] efs (\<lambda>ef. wp s UNIV ef (\<lambda>_. upred_emp)))))))))))"
-by auto            
+by auto
 
+abbreviation WP :: "expr \<Rightarrow> (val \<Rightarrow> iprop) \<Rightarrow> iprop" ("WP _ {{ _ }}") where
+  "WP e {{ \<Phi> }} \<equiv> wp NotStuck {} e \<Phi>"
+
+text \<open>
+  First we show that all basic properties of wp hold for inputs in the domain, then we 
+  always assume all values to lie in the domain.
+\<close>
+context begin
+lemma wp_value_fupd: 
+  assumes "wp_dom (s, E, Val v, P)"
+  shows "wp s E (of_val v) P \<stileturn>\<turnstile> \<Turnstile>{E}=> P v"
+  by (auto simp: wp.psimps[OF assms])
+
+lemma wp_value: 
+  assumes "wp_dom (s, E, Val v, P)"
+  shows "P v \<turnstile> wp s E (Val v) P"
+  by (auto simp: wp.psimps[OF assms] fupd_intro upred_wand_holdsE)
+
+lemma wp_strong_mono: 
+  assumes "wp_dom (s1, E1, e, P)" "wp_dom (s2, E2, e, Q)"
+    "s1 \<le> s2" "E1 \<subseteq> E2" 
+  shows "wp s1 E1 e P -\<^emph> (\<forall>\<^sub>u v. (P v ={E2}=\<^emph> Q v)) -\<^emph> wp s2 E2 e Q"
+  apply (rule upred_wand_holds2I)
+  sorry
+
+lemma wp_lift_step_fupdN: 
+assumes "HeapLang.to_val e1 = None"
+shows "(\<forall>\<^sub>u \<sigma>1 \<kappa> \<kappa>s. ((state_interp \<sigma>1 (\<kappa>@\<kappa>s)) ={E,Set.empty}=\<^emph>
+  ((\<upharpoonleft>(case s of NotStuck \<Rightarrow> red e1 \<sigma>1 | _ \<Rightarrow> True)) \<^emph>
+  (\<forall>\<^sub>u e2 \<sigma>2 efs. ((\<upharpoonleft>(prim_step e1 \<sigma>1 \<kappa> e2 \<sigma>2 efs)) ={Set.empty}\<triangleright>=\<^emph> 
+    (\<Turnstile>{Set.empty,E}=> ((state_interp \<sigma>2 \<kappa>s) \<^emph>
+      (wp s E e2 \<Phi>) \<^emph> ([\<^emph>\<^sub>l:] efs (\<lambda>ef. wp s UNIV ef (\<lambda>_. upred_emp))))))))))
+   \<turnstile> wp s E e1 \<Phi>"
+ sorry (* Axiomatized as reasoning with wp_dom is quite hard.*)
+end   
 end
