IrisCore/COFEs.thy
@@ -13,11 +13,84 @@ class cofe = ofe +
   fixes lim :: "('a::ofe) chain \<Rightarrow> 'a"
   assumes core_compl: "n_equiv n (lim c) (Rep_chain c n)"
 
+definition discrete_lim :: "('a::discrete chain) \<Rightarrow> 'a" where
+  "discrete_lim c = Rep_chain c 0"
+
+lemma discrete_cofe: "n_equiv n (discrete_lim c) (Rep_chain c n)"
+  unfolding discrete_lim_def by transfer (metis d_equiv nat_le_linear)
+
+subsubsection \<open>Banach's fixed-point\<close>
+
+definition fixpoint_chain :: "('a::ofe,'a) contr \<Rightarrow> 'a chain" where
+  "fixpoint_chain f = Abs_chain (\<lambda>n. Nat.compower (Rep_contr f) (Suc n) (SOME (x::'a). True))"
+
+definition fixpoint :: "('a::cofe,'a) contr \<Rightarrow> 'a" where
+  "fixpoint f = lim (fixpoint_chain f)"
+
+lemma fp_chain:"(\<lambda>n. Nat.compower (Rep_contr (f::('a::cofe,'a) contr)) (Suc n) x) \<in>
+  {c. \<forall>n m. n\<le>m \<longrightarrow> n_equiv n (c m) (c n)}"
+  apply auto apply transfer 
+  subgoal for n m f x
+proof (induction n arbitrary: m)
+  case 0
+  then show ?case by (auto intro: contractiveE)
+next
+  case (Suc n)
+  then have "n \<le> (m-1)" by simp
+  then obtain m' where m': "m' = m-1" by simp
+  then have f_m': "f ((f^^m') x) = (f^^m) x" apply auto
+    by (metis One_nat_def Suc.prems(1) Suc_le_D comp_def diff_Suc_1 funpow.simps(2))
+  from m' \<open>n\<le>(m-1)\<close> have "n\<le>m'" by simp
+  show ?case apply (rule contractive_Suc[OF Suc(3)])
+  using Suc(1)[OF \<open>n\<le>m'\<close> Suc(3)] by (auto simp: f_m')
+qed
+done
+
+lemma fixpoint_unfold: "ofe_eq (fixpoint f) (Rep_contr f (fixpoint f))" 
+apply (auto simp: ofe_limit fixpoint_def)
+subgoal for n
+apply (induction n)
+subgoal
+  apply (subst ofe_trans_eqL[OF core_compl])
+  apply (auto simp: fixpoint_chain_def Abs_chain_inverse[OF fp_chain, simplified])
+  using Rep_contr contractive_zero by blast
+subgoal for n'
+  unfolding ofe_trans_eqL[OF core_compl]
+  apply (auto simp: fixpoint_chain_def Abs_chain_inverse[OF fp_chain, simplified])
+  by (auto simp: ofe_trans_eqR[OF core_compl] Abs_chain_inverse[OF fp_chain, simplified] ofe_refl
+    intro!: contractive_Suc[of "Rep_contr f"])
+  done
+done
+
+lemma banachs_fixes_point2: "ofe_eq x (Rep_contr f x) \<Longrightarrow> ofe_eq x (fixpoint f)"
+apply (auto simp: ofe_limit)
+subgoal for n
+proof (induction n)
+  case 0
+  then have x0: "n_equiv 0 x (Rep_contr f x)" by simp
+  show ?case 
+    by (auto simp: fixpoint_def fixpoint_chain_def ofe_trans_eqR[OF core_compl] 
+      Abs_chain_inverse[OF fp_chain, simplified] ofe_trans_eqL[OF x0] intro:
+      contractive_zero)
+next
+  case (Suc n)
+  then have IH: "n_equiv n x (fixpoint f)" by simp
+  from Suc(2) have x_Sn: "n_equiv (Suc n) x (Rep_contr f x)" by simp
+  show ?case apply (auto simp: ofe_trans_eqL[OF x_Sn] ofe_trans_eqR[OF ofe_eq_equiv[OF fixpoint_unfold]])
+  apply (rule contractive_Suc[of "Rep_contr f"])
+  by (auto simp: IH)
+qed
+done
+
+subsection \<open>COFE instances\<close>
+
+subsubsection \<open>Unit type cofe\<close>
 instantiation unit :: cofe begin
 definition lim_unit :: "unit chain \<Rightarrow> unit" where [simp]: "lim_unit _ = ()"
 instance by standard (simp add: n_equiv_unit_def)
 end
 
+subsubsection \<open>Option type cofe\<close>
 lift_definition option_chain :: "'a::ofe option chain \<Rightarrow> 'a \<Rightarrow> 'a chain" is
   "\<lambda>c x n. case c n of Some y \<Rightarrow> y | None \<Rightarrow> x" 
   by (auto simp: ofe_refl n_equiv_option_def split: option.splits) fastforce+
@@ -37,6 +110,7 @@ instance proof
 qed
 end
 
+subsubsection \<open>Later type ofe\<close>
 lift_definition later_chain :: "'a::ofe later chain \<Rightarrow> 'a chain" is
   "\<lambda>c n. later_car (Rep_chain c (Suc n))" 
   by transfer (metis Suc_le_mono add_diff_cancel_left' n_equiv_later_def nat.discI plus_1_eq_Suc)
@@ -52,13 +126,6 @@ instance proof
 qed
 end
 
-definition discrete_lim :: "('a::discrete chain) \<Rightarrow> 'a" where
-  "discrete_lim c = Rep_chain c 0"
-
-lemma discrete_cofe: "n_equiv n (discrete_lim c) (Rep_chain c n)"
-  unfolding discrete_lim_def by transfer (metis d_equiv nat_le_linear)
-
-subsection \<open>COFE instances\<close>
 subsubsection \<open>Product type COFE\<close>
 lift_definition chain_map :: "('a::ofe -n> 'b::ofe) \<Rightarrow> 'a chain \<Rightarrow> 'b chain" is
   "\<lambda>f c n. f (Rep_chain c n)" by transfer (simp add: non_expansive_def)
