SpanningTree/Spanning.thy
@@ -35,9 +35,11 @@ definition span :: val where "span \<equiv>
 subsubsection \<open>Proofs\<close>
 lemma wp_try_mark:
 assumes "x\<in>dom g" 
-shows "graph_ctxt g Mrk \<^emph> own_graphUR q Map.empty \<^emph> cinv_own k \<turnstile>
-  wp (App (of_val try_mark) (of_val #[x])) (\<lambda>v. 
+shows "(graph_ctxt g Mrk) \<^emph> (own_graphUR q Map.empty) \<^emph> (cinv_own k) \<turnstile>
+  WP (App (of_val try_mark) (of_val #[x])) 
+  {{ \<lambda>v. 
     ((\<upharpoonleft>(v=#[True])) \<^emph> (\<exists>\<^sub>u u. (((\<upharpoonleft>(g x = Some u)) \<^emph> own_graphUR q (x [\<mapsto>\<^sub>g] u)) \<^emph> is_marked x \<^emph> cinv_own k)))
-    \<or>\<^sub>u ((\<upharpoonleft>(v=#[False])) \<^emph> own_graphUR q Map.empty \<^emph> is_marked x \<^emph> cinv_own k))"
+    \<or>\<^sub>u ((\<upharpoonleft>(v=#[False])) \<^emph> own_graphUR q Map.empty \<^emph> is_marked x \<^emph> cinv_own k) 
+  }}"
 sorry
 end
